fix logic

main.c
@@ -2,7 +2,7 @@
 #include <stdio.h>
 #include "Slice.h"
 
-void print_sliced (uint32_t *u32_array, uint32_t u32_array_length, uint32_t from, uint32_t to) {
+void print_slice (uint32_t *u32_array, uint32_t u32_array_length, uint32_t from, uint32_t to) {
   uint32_t *sliced = (uint32_t *)malloc(u32_array_length * sizeof(uint32_t));
   uint32_t sliced_length = slice(u32_array, u32_array_length, sliced, from, to);
   printf("[");
@@ -19,8 +19,8 @@ void print_sliced (uint32_t *u32_array, uint32_t u32_array_length, uint32_t from
 int main() {
   uint32_t u32_array[] = {0, 1, 2, 3, 4};
   uint32_t u32_array_length = sizeof(u32_array) / sizeof(uint32_t);
-  print_sliced(u32_array, u32_array_length, 0, 5);
-  print_sliced(u32_array, u32_array_length, 2, 4);
-  print_sliced(u32_array, u32_array_length, 5, 0);
+  print_slice(u32_array, u32_array_length, 0, 5);
+  print_slice(u32_array, u32_array_length, 2, 4);
+  print_slice(u32_array, u32_array_length, 5, 0);
   return 0;
 }
